src/named/Tactics.v
@@ -1,0 +1,299 @@
+(*********************************************
+A partial recognizer for well-formed languages
+**********************************************)
+
+
+Require Import mathcomp.ssreflect.all_ssreflect.
+Set Implicit Arguments.
+Unset Strict Implicit.
+Unset Printing Implicit Defensive.
+Set Bullet Behavior "Strict Subproofs".
+
+From Utils Require Import Utils.
+From Named Require Import Exp Rule Core.
+
+From Ltac2 Require Import Ltac2.
+Require Ltac2.List Ltac2.Option Ltac2.Std.
+(*TODO: copied from stdlib; need to update version?*)
+Ltac2 of_goal () := Fresh.Free.of_ids (List.map (fun (id, _, _) => id) (Control.hyps ())).
+
+Ltac2 in_goal id := Fresh.fresh (of_goal ()) id.
+
+Ltac2 fresh s := in_goal (Option.get (Ident.of_string s)).
+
+(*
+tests whether two terms are equal,
+unifying evars as necessary.
+EFFECT: adds a = b as a hypothesis if true,
+possibly instantiating evars in the process
+ *)
+Ltac2 eequal a b :=
+  Control.plus
+    (fun () =>
+       let heq := fresh "Heq" in
+       assert ($a = $b)>[solve[f_equal; eauto]|]; true)
+    (fun _ => false).
+
+(* Attempts to clear a goal of the form
+   'a \in l', unifying evars as necessary *)
+Ltac2 rec unify_in () :=
+  match! goal with
+    [|- is_true (?r \in ?r'::?l)] =>
+    rewrite in_cons;
+    ltac1:(apply /orP);
+    match eequal r r' with
+    | true => left;ltac1:(by apply /eqP)
+    | false => right; unify_in()
+    end
+  end.
+
+Require Import String.
+  
+Ltac2 try f :=
+  Control.enter
+    (fun () => Control.plus f (fun _ => ())).
+
+Ltac2 all_red_flags :=
+  { Std.rBeta := true;
+  Std.rMatch := true;
+  Std.rFix := true;
+  Std.rCofix := true;
+  Std.rZeta := true;
+  Std.rDelta := true;
+  Std.rConst := []
+}.
+
+Ltac2 goal_lang () :=
+  lazy_match! goal with
+  | [|- le_term ?l _ _ _ _] => l
+  | [|- le_sort ?l _ _ _] => l
+  | [|- wf_term ?l _ _ _] => l
+  | [|- wf_sort ?l _ _] => l
+  | [|- wf_rule ?l _] => l
+  | [|- wf_ctx ?l _] => l
+end.
+
+
+
+(* taken from https://github.com/coq/coq/issues/11641 *)
+Ltac2 my_change2 (a : constr) (b : constr) :=
+  ltac1:( a b |- change a with b ) (Ltac1.of_constr a) (Ltac1.of_constr b).
+
+Ltac2 unify_eq () :=
+  match! goal with
+    [|- ?a = ?b] =>
+    solve[f_equal; eauto]
+  end.
+
+Ltac2 Type exn ::= [JudgmentMismatchExn(constr, constr)].
+Ltac2 apply_rule (name : constr) :=
+  let l := goal_lang () in
+  (* TODO: make d an evar so it isn't silently returned?*)
+  let d := constr:(sort_rule [::]) in
+  let r := Std.eval_cbv all_red_flags
+           constr:(named_list_lookup $d $l $name) in
+  lazy_match! r with
+  | sort_rule ?c' =>
+    lazy_match! goal with
+    | [|- wf_sort ?l ?c ?t] =>
+      eapply (@wf_sort_by $l $c $name) >
+      [ unify_in ()|]
+    | [|- ?j] =>
+      Control.zero
+        (JudgmentMismatchExn constr:(($name,$r)) j)
+    end
+  | term_rule ?c' ?t' =>
+    lazy_match! goal with
+    | [|- wf_term ?l ?c ?e ?t] =>
+      ltac1:(l c e t t'|-
+             let s := fresh "s" in
+             evar (s : subst);
+             replace (wf_term l c e t) with
+                (wf_term l c e t'[/s/]);
+            unfold s;
+            clear s
+            ) (Ltac1.of_constr l)
+              (Ltac1.of_constr c)
+              (Ltac1.of_constr e)
+              (Ltac1.of_constr t)
+              (Ltac1.of_constr t') >
+            [ eapply (@wf_term_by $l $c $name) >
+              [ unify_in () |]
+            | unify_eq()]
+    | [|- ?j] =>
+      Control.zero
+        (JudgmentMismatchExn constr:(($name,$r)) j)
+    end
+end.
+
+Check wf_sort_by.
+Goal wf_term [:: [:| |- "foo" : #"bar"]] [::] (con "foo" [::])
+(srt "bar" [::]).
+Proof.
+  
+  apply_rule constr:("foo"%string).
+  
+  admit.
+  cbv.
+  unfold substable_sort.
+  f_equal; eauto.
+  unify_eq ().
+  
+TODO: deconstruct subst automatically based on c'  
+  
+
+(* TODO: generalize over key, value types? *)
+Ltac2 Type rec FinMap :=
+  [ MapEmpty
+  | MapCons (constr (*Coq string*), constr, FinMap)].
+
+Ltac2 Type exn ::= [EmptyMapLookupExn].
+Ltac2 rec map_lookup n m :=
+  match m with
+  | MapEmpty => Control.zero EmptyMapLookupExn
+  | MapCons n' v m' =>
+    match Constr.equal n' n with
+    | true => v
+    | false => map_lookup n m'
+    end
+  end.
+
+
+
+(* Computes a map that has all mappings from both,
+   or throws if none exists
+TODO: optimize representation for this operation
+ *)
+Ltac2 Type exn ::= [MapMergeExn(constr, constr)].
+Ltac2 rec map_merge m1 m2 :=
+  match m1 with
+  | MapEmpty => m2
+  | MapCons k v1 m1' =>
+    MapCons k v1
+            (Control.plus
+               (fun _ => let v2 := map_lookup k m2 in
+                match Constr.equal v1 v2 with
+                | true => map_merge m1' m2
+                | false => Control.zero (MapMergeExn v1 v2)
+                end)
+               (fun ex =>
+                  match ex with
+                  | EmptyMapLookupExn => map_merge m1' m2
+                  | _ => Control.zero ex
+                  end))
+  end.
+
+Ltac2 Type exn ::= [DomainExn(constr, constr, constr)].
+Ltac2 dom_exn c t := DomainExn c (Constr.type c) t.
+(* TODO: do this for coq strings*)
+Ltac2 rec int_of_nat c :=
+  match! c with
+  | 0 => 0
+  | S ?c' => Int.add 1 (int_of_nat c')
+  | _ => Control.throw (dom_exn c constr:(nat)) 
+  end.
+
+Ltac2 Type exn ::= [ExpMatchExn(constr, constr)].
+Ltac2 rec exp_match (p : constr) e :=
+  match! p with
+  | var ?x => MapCons (int_of_nat x) e MapEmpty
+  | con ?pn ?ps =>
+    match! e with
+    | con ?n ?s =>
+      match Constr.equal pn n with
+      | true => subst_match ps s
+      | false => Control.throw (ExpMatchExn p e)
+      end
+    | var _ => Control.throw (ExpMatchExn p e)
+    | _ => Control.throw (dom_exn e constr:(exp))
+      (* TODO: need to handle evars*)
+    end
+  | _ => Control.throw (dom_exn p constr:(exp))
+  end
+with subst_match p s :=
+    match! p with
+    | [::] => match! s with [::] => MapEmpty end
+    | ?pe::?p' =>
+      match! s with
+      | ?e::?s' =>
+        map_merge (exp_match pe e) (subst_match p' s')
+      | [::] => Control.throw (ExpMatchExn p s)
+      end
+    end.
+
+Ltac2 Eval (exp_match constr:(var 1) constr:(var 2)).
+Ltac2 Eval
+      (exp_match constr:(con 1 [:: var 2; var 2])
+                          constr:(con 1 [:: (con 2 [::]); (con 2 [::])])).
+
+
+(* assumes idx <= size 
+   TODO: how to handle terms that aren't listed?
+   evar?
+*)
+Ltac2 subst_of_map m size :=
+  let rec som idx acc :=
+      match Int.equal idx size with
+      | true => acc
+      | false =>
+        let v := map_lookup idx m in
+        som (Int.add idx 1) constr:($v::$acc)
+      end in
+  som 0 constr:(@nil exp).
+
+Ltac2 Eval (subst_of_map
+              (MapCons 2 constr:(var 3)
+              (MapCons 0 constr:(var 1)
+              (MapCons 1 constr:(var 2) MapEmpty)))) 3.
+
+Ltac2 max n m :=
+  match Int.gt n m with
+  | true => n
+  | false => m
+  end.
+
+Ltac2 rec min_subst_size m :=
+  match m with
+  | MapEmpty => 0
+  | MapCons n _ m' =>
+    max (Int.add n 1) (min_subst_size m')
+  end.
+
+Require Import Ltac2.Notations.
+
+Ltac2 rec unify_in () :=
+  match! goal with
+    [|- is_true (?r \in ?r'::?l)] =>
+    rewrite in_cons;
+    ltac1:(apply /orP);
+    Control.plus
+      (fun () => left;ltac1:(apply /eqP; by f_equal))
+      (fun _ =>
+         right; unify_in ())
+end.
+
+Ltac2 apply_term_rule n :=
+  match! goal with
+    [|- le_term ?l ?c ?t ?e1 ?e2 ]=>
+    match! Std.eval_hnf constr:(nth_level (sort_rule [::]) $l $n) with
+      term_le _ ?pe1 ?pe2 ?pt =>
+      let m := subst_match constr:([:: $pt; $pe1; $pe2])
+                           constr:([:: $t; $e1; $e2]) in
+      let s := subst_of_map m (min_subst_size m) in
+      my_change2
+        constr:(le_term $l $c $t $e1 $e2)
+        constr:(le_term $l $c $pt[/$s/] $pe1[/$s/] $pe2[/$s/]);
+      eapply le_term_subst;
+      Control.enter
+        (fun () =>
+           match! goal with
+           | [|- le_term _ _ _ _ _] =>
+             eapply le_term_by;
+             unify_in ()
+           | [|- le_subst _ _ _ _ _] => ()
+           | [|- _] => Control.throw Match_failure
+           end)
+    end
+end.
+
+
